Introduce UOp for all index arities (#96)
* UserOp full

* Fix

* Fixes

CpcMini/Logos.lean
@@ -58,11 +58,29 @@ inductive UserOp : Type where
 
 deriving Repr, DecidableEq, Inhabited, Ord
 
+inductive UserOp1 : Type where
+  | None : UserOp1
+
+deriving Repr, DecidableEq, Inhabited, Ord
+
+inductive UserOp2 : Type where
+  | None : UserOp2
+
+deriving Repr, DecidableEq, Inhabited, Ord
+
+inductive UserOp3 : Type where
+  | None : UserOp3
+
+deriving Repr, DecidableEq, Inhabited, Ord
+
 mutual
 
 /- Term definition -/
 inductive Term : Type where
   | UOp : UserOp -> Term
+  | UOp1 : UserOp1 -> Term -> Term
+  | UOp2 : UserOp2 -> Term -> Term -> Term
+  | UOp3 : UserOp3 -> Term -> Term -> Term -> Term
   | __eo_List : Term
   | __eo_List_nil : Term
   | __eo_List_cons : Term
